Weidenbach_Book/IsaSAT/IsaSAT_Simplify_Forward_Subsumption_LLVM.thy
@@ -10,6 +10,61 @@ begin
 no_notation WB_More_Refinement.fref (\<open>[_]\<^sub>f _ \<rightarrow> _\<close> [0,60,60] 60)
 no_notation WB_More_Refinement.freft (\<open>_ \<rightarrow>\<^sub>f _\<close> [60,60] 60)
 
+definition incr_forward_subsumed_st  :: \<open>_\<close> where
+  \<open>incr_forward_subsumed_st S = (set_stats_wl_heur (incr_forward_subsumed (get_stats_heur S)) S)\<close>
+
+definition incr_forward_strengthened_st  :: \<open>_\<close> where
+  \<open>incr_forward_strengthened_st S = (set_stats_wl_heur (incr_forward_strengethening (get_stats_heur S)) S)\<close>
+
+lemma incr_forward_subsumed_st_alt_def: \<open>incr_forward_subsumed_st S = (
+  let (stats, S) = extract_stats_wl_heur S; stats = incr_forward_subsumed stats in
+    update_stats_wl_heur stats S
+    )\<close> and
+  incr_forward_strengthened_st_alt_def: \<open>incr_forward_strengthened_st S = (
+  let (stats, S) = extract_stats_wl_heur S; stats = incr_forward_strengethening stats in
+    update_stats_wl_heur stats S
+    )\<close>
+  by (auto simp: isa_push_to_occs_list_st_def state_extractors incr_forward_subsumed_st_def incr_forward_strengthened_st_def
+         split: isasat_int_splits) 
+
+sepref_def Subsumption_Stats_incr_strengthening_impl
+  is \<open>RETURN o Subsumption_Stats_incr_strengthening\<close>
+  :: \<open>subsumption_stats_assn\<^sup>d \<rightarrow>\<^sub>a subsumption_stats_assn\<close>
+  unfolding Subsumption_Stats_incr_strengthening_def subsumption_stats_assn_def
+  by sepref
+
+sepref_def incr_forward_strengethening_impl
+  is \<open>RETURN o incr_forward_strengethening\<close>
+  :: \<open>isasat_stats_assn\<^sup>d \<rightarrow>\<^sub>a isasat_stats_assn\<close>
+  unfolding incr_forward_strengethening_def stats_code_unfold
+  by sepref
+
+sepref_def incr_forward_strengthened_st_impl
+  is \<open>RETURN o incr_forward_strengthened_st\<close>
+  :: \<open>isasat_bounded_assn\<^sup>d \<rightarrow>\<^sub>a isasat_bounded_assn\<close>
+  unfolding incr_forward_strengthened_st_alt_def
+  by sepref
+
+sepref_def Subsumption_Stats_incr_subsumed_impl
+  is \<open>RETURN o Subsumption_Stats_incr_subsumed\<close>
+  :: \<open>subsumption_stats_assn\<^sup>d \<rightarrow>\<^sub>a subsumption_stats_assn\<close>
+  unfolding Subsumption_Stats_incr_subsumed_def subsumption_stats_assn_def
+  by sepref
+
+sepref_def incr_forward_subsumed_impl
+  is \<open>RETURN o incr_forward_subsumed\<close>
+  :: \<open>isasat_stats_assn\<^sup>d \<rightarrow>\<^sub>a isasat_stats_assn\<close>
+  unfolding incr_forward_subsumed_def stats_code_unfold
+  by sepref
+
+sepref_def incr_forward_subsumed_st_impl
+  is \<open>RETURN o incr_forward_subsumed_st\<close>
+  :: \<open>isasat_bounded_assn\<^sup>d \<rightarrow>\<^sub>a isasat_bounded_assn\<close>
+  unfolding incr_forward_subsumed_st_alt_def
+  by sepref
+
+sepref_register incr_forward_subsumed_st incr_forward_strengthened_st
+
 definition clause_size_sort_clauses_raw :: \<open>arena \<Rightarrow> vdom \<Rightarrow> nat \<Rightarrow> nat \<Rightarrow> nat list nres\<close> where
   \<open>clause_size_sort_clauses_raw arena N = pslice_sort_spec idx_clause_cdom clause_size_less arena N\<close>
 
@@ -626,6 +681,7 @@ sepref_def isa_strengthen_clause_wl2_impl
   :: \<open>sint64_nat_assn\<^sup>k *\<^sub>a sint64_nat_assn\<^sup>k *\<^sub>a unat_lit_assn\<^sup>k *\<^sub>a isasat_bounded_assn\<^sup>d \<rightarrow>\<^sub>a isasat_bounded_assn\<close>
   unfolding isa_strengthen_clause_wl2_def mop_arena_status_st_def[symmetric]
     mop_arena_length_st_def[symmetric]
+  apply (subst incr_forward_strengthened_st_def[symmetric])+
   by sepref
 
   
@@ -639,6 +695,7 @@ sepref_def isa_subsume_or_strengthen_wl_impl
   is \<open>uncurry2 isa_subsume_or_strengthen_wl\<close>
   :: \<open>sint64_nat_assn\<^sup>k *\<^sub>a subsumption_assn\<^sup>k *\<^sub>a isasat_bounded_assn\<^sup>d \<rightarrow>\<^sub>a isasat_bounded_assn\<close>
   unfolding isa_subsume_or_strengthen_wl_def subsumption_cases_split mop_arena_status_st_def[symmetric]
+    incr_forward_subsumed_st_def[symmetric]
   by sepref
 
 sepref_def isa_forward_subsumption_one_wl_impl
